code/experimental/SPARKLE/dist/test.c
@@ -1,0 +1,51 @@
+#include <inttypes.h>
+#include <stdio.h>
+#include <stdlib.h>
+#include <string.h>
+#include <sys/types.h>
+#include <sys/stat.h>
+#include <fcntl.h>
+#include <unistd.h>
+#include <time.h>
+#include <stdbool.h>
+#include "test_helpers.h"
+
+#include "Hacl_Impl_Sparkle.h"
+#include "test_implementation.c"
+
+
+#include <stdint.h>
+#include <string.h>
+#include <stdint.h>
+
+
+
+
+
+int main(int argc, char const *argv[])
+{
+
+	uint32_t* input = (uint32_t*) malloc (sizeof (uint32_t) * 8);
+	uint32_t* expected_output = (uint32_t*) malloc (sizeof (uint32_t) * 8);
+	memcpy(input, expected_output, 32);
+	sparkle(expected_output, 4, 32);
+
+
+	uint8_t* input_hacl = (uint8_t*) malloc (sizeof (uint8_t) * 32);
+	uint8_t* output_hacl = (uint8_t*) malloc (sizeof (uint8_t) * 32);
+
+
+	Hacl_Impl_Sparkle_sparkle256(32, input_hacl, output_hacl);
+
+	printf("%s\n", "Expected input");
+	compare_and_print(32, input, input);
+	printf("%s\n", "Expected output");
+	compare_and_print(32, expected_output, expected_output);
+
+	printf("%s\n", "Input");
+	compare_and_print(32, input_hacl, input_hacl);
+	printf("%s\n", "Output");
+	compare_and_print(32, output_hacl, output_hacl);
+
+	return 0;
+}
