code/experimental/SPARKLE/dist/test_implementation.c
@@ -1,0 +1,60 @@
+#define MAX_BRANCHES 8
+#define ROT(x , n) ((( x) >> (n )) | (( x) << (32 - (n))) )
+#define ELL(x) ( ROT ((( x ) ^ (( x ) << 16) ) , 16) )
+
+// Round constants
+static const uint32_t RCON [ MAX_BRANCHES ] = {
+	0xB7E15162 , 0xBF715880 , 0x38B4DA56 , 0x324E7738 ,
+	0xBB1185EB , 0x4F7C7B57 , 0xCFBFA1C8 , 0xC2B3293D};
+
+
+void sparkle ( uint32_t * state , int nb , int ns )
+{
+
+ int i , j; // Step and branch counter
+ uint32_t rc , tmpx , tmpy , x0 , y0 ;
+
+ for (i = 0; i < ns ; i ++) {
+	 // Counter addition
+	 state [1] ^= RCON [i % MAX_BRANCHES];
+	 state [3] ^= i;
+
+	 // ARXBox layer
+	 for (j = 0; j < 2 * nb ; j += 2) {
+		 rc = RCON [j >> 1];
+		 state [j] += ROT ( state [j + 1] , 31) ;
+		 state [j +1] ^= ROT ( state [j], 24) ;
+		 state [j] ^= rc ;
+		 state [j] += ROT ( state [j + 1] , 17) ;
+		 state [j +1] ^= ROT ( state [j], 17) ;
+		 state [j] ^= rc ;
+		 state [j] += state [j +1];
+		 state [j +1] ^= ROT ( state [j], 31) ;
+		 state [j] ^= rc ;
+		 state [j] += ROT ( state [j + 1] , 24) ;
+		 state [j +1] ^= ROT ( state [j ], 16) ;
+		 state [j] ^= rc ;}
+
+	 // Linear layer
+	 tmpx = x0 = state [0];
+	 tmpy = y0 = state [1];
+
+	 for (j = 2; j < nb ; j += 2) {
+		 tmpx ^= state [j ];
+		 tmpy ^= state [j +1];}
+
+	 tmpx = ELL ( tmpx );
+	 tmpy = ELL ( tmpy );
+	 
+	 for (j = 2; j < nb ; j += 2) {
+		 state [j -2] = state [j+ nb ] ^ state [j] ^ tmpy ;
+		 state [j+ nb ] = state [ j ];
+		 state [j -1] = state [j+ nb +1] ^ state [j +1] ^ tmpx ;
+		 state [j+ nb +1] = state [j +1];}
+
+
+	 state [nb -2] = state [ nb ] ^ x0 ^ tmpy ;
+	 state [ nb ] = x0 ;
+	 state [nb -1] = state [ nb +1] ^ y0 ^ tmpx ;
+	 state [ nb +1] = y0; }
+}
